src/Parsers/Refinement/SharpenedABStar.v
@@ -1,7 +1,6 @@
 (** Sharpened ADT for (ab)* *)
 Require Import ADTSynthesis.Parsers.Refinement.Tactics.
 Require Import ADTSynthesis.Parsers.Grammars.ABStar.
-
 Set Implicit Arguments.
 
 Section IndexedImpl.
@@ -22,3 +21,28 @@ Section IndexedImpl.
   Defined.
 
 End IndexedImpl.
+
+Require Import ADTSynthesis.Parsers.ParserFromParserADT.
+Require Import ADTSynthesis.Parsers.ParserImplementation.
+Require Import ADTSynthesis.ADT.ComputationalADT.
+
+Definition ab_star_parser : String.string -> bool.
+Proof.
+  refine (fun s => has_parse (parser (adt_based_splitter ComputationalSplitter)) _).
+  pose (cConstructors (projT1 ComputationalSplitter) {| StringBound.bindex := "new" |} s).
+  Require Import StringLike.Core StringLike.String.
+  simpl.
+  pose .
+  simpl in c.
+  unfold cConstructorType in *.
+
+lazy.
+ (s, (0, String.length s))).
+    simpl in b.
+Require Import StringLike.Core.
+simpl in b.
+Set Printing All.
+
+
+Check ab_star_parser.
+Check .
